formula_prices_list.thy
@@ -15,13 +15,69 @@ The equivalences of the spectrum (or their modal-logical characterizations) can 
 equivalence $X$ is characterized by the HML formulas with prices less then or equal to a \textit{X-price bound} $e_X$.
 We use the six dimensions from (energy games) to characterize the notions of equivalence we are interested in (In figure xx oder so umschreiben).
 Intuitively, the dimensions can be described as follows:\\
-1. Observations\\
-...
-...\\ \<close>
+1. Formula modal depth of observations: How many modal operations $\langle \alpha \rangle$ may one pass when descending the syntax tree. (Algebraic laws for nondeterminism and concurrency)(Operational and algebraic semantics of concurrent processes)\\
+2. Formula nesting depth of conjunctions: How often may one pass a conjunction?
+3. Maximal modal depth of deepest positive clauses in conjunctions: The modal depth of the deepest positive clause within a conjunction ??!!!!
+4. Maximal modal depth of other positive clauses in conjunctions: The modal depth of the other positive clauses... !!??!!
+5. Maximal modal depth of negative clauses in conjunctions: ... self explanatory...
+6. Formula nesting depth of negations: How many negations may be visited when descending? This is sometimes called the number of ``alternations'' between [] and <>.(Citation suchen, warum?)
+\<close>
 
-subsubsection \<open>Formula Prices\<close>
+subsubsection \<open>Definition 2.1 (Formula Prices)\<close>
 text \<open>The \textit{expressiveness price} $\text{expr}: \text{HML}[\Sigma] \rightarrow (\mathbb{N} \cup \{\infty\})^6$ of a formula is defined recursively, similar to energy games:
-TODO: $\text{expr}$ function \\\\
+
+The expressiveness price $\text{expr} : \text{HML}[\Sigma] \rightarrow (\mathbb{N \cup \infty})^6$ of a formula interpreted as $6 \times 1$-dimensional vectors is defined recursively by:
+
+\[
+\text{expr}(\langle a \rangle \varphi) :=
+\begin{pmatrix}
+1 + \text{expr}_1(\varphi) \\
+\text{expr}_2(\varphi) \\
+\text{expr}_3(\varphi) \\
+\text{expr}_4(\varphi) \\
+\text{expr}_5(\varphi) \\
+\text{expr}_6(\varphi) \\
+\end{pmatrix}
+\]
+
+\[
+\text{expr}(\neg \varphi) := 
+\begin{pmatrix}
+\text{expr}_1(\varphi) \\
+\text{expr}_2(\varphi) \\
+\text{expr}_3(\varphi) \\
+\text{expr}_4(\varphi) \\
+\text{expr}_5(\varphi) \\
+1 + \text{expr}_6(\varphi) \\
+\end{pmatrix}
+\]
+
+\[
+\text{expr}\left( \bigwedge_{i \in I} \psi_i \right) := 
+\begin{pmatrix}
+0 \\
+1 + \sup_{i \in I} \text{expr}_2(\psi_i) \\
+\sup_{i \in \text{Pos}} \text{expr}_1(\psi_i) \\
+\sup_{i \in \text{Pos} \backslash \mathcal{R}} \text{expr}_1(\psi_i) \\
+\sup_{i \in \text{Neg}} \text{expr}_1(\psi_i) \\
+0 \\
+\end{pmatrix}
+\]
+
+where:
+
+$\text{Neg} := \{i \in I \, | \, \exists \varphi'_i. \psi_i = \neg \varphi'_i\}$
+
+$\text{Pos} := I \setminus \text{Neg}$
+
+$\mathcal{R} := \left\{
+\begin{aligned}
+&\varnothing \text{ if } \text{Pos} = \varnothing, \\
+&\{ r \} \text{ for some } r \in \text{Pos} \text{ where } \text{expr}_1(\psi_r) \text{ maximal for Pos}
+\end{aligned}
+\right.$
+
+Our Isabelle-definition of HML makes it very easy to derive the sets Pos and Neg, by \<open>\<Phi> ` I\<close> and \<open>\<Phi> ` J\<close> respectively.
 
 Remark: Infinity is included in our definition, due to infinite branching conjunctions. Supremum over infinite set wird zu unendlich.\<close>
 
@@ -33,12 +89,27 @@ direct\_expr definition,
 einzelne dimensionen,
 lemma direct\_expr = expr...\<close>
 
+text \<open>Formally, the \textit{modal depth} $\textsf{expr}_1$ of a formula $\varphi$ is defined recursively by:
+
+\begin{align*}
+    \text{if } \varphi &= \langle a \rangle \psi \quad \text{ with } a \in \Sigma \\
+    &\text{then } \textsf{expr}_1(\varphi) = 1 + \textsf{expr}_1(\psi) \\
+    \text{if } \varphi &= \bigwedge_{i \in I} \{ \psi_1, \psi_2, \ldots \} \\
+    &\text{then } \textsf{expr}_1(\varphi) = \sup(\textsf{expr}_1(\psi_i)) \\
+    \text{if } \psi &= \neg \varphi \\
+    &\text{then } \textsf{expr}_1(\psi) = \textsf{expr}_1(\varphi)
+\end{align*}
+
+\<close>
+
 primrec expr_1 :: "('a, 's)hml \<Rightarrow> enat"
   where
 expr_1_tt: \<open>expr_1 TT = 0\<close> |
 expr_1_conj: \<open>expr_1 (hml_conj I J \<Phi>) = Sup ((expr_1 \<circ> \<Phi>) ` I \<union> (expr_1 \<circ> \<Phi>) ` J)\<close> |
 expr_1_pos: \<open>expr_1 (hml_pos \<alpha> \<phi>) = 
   1 + (expr_1 \<phi>)\<close>
+
+text \<open>With the help of the modal depth we can derive Pos$\backslash$R in Isabelle:\<close>
 
 fun pos_r :: "('a, 's)hml set \<Rightarrow> ('a, 's)hml set"
   where
@@ -48,8 +119,7 @@ let max_val = (Sup (expr_1 ` xs));
   xs_new = xs - {max_elem}
 in xs_new)"
 
-lemma pos_r_subs: "pos_r (\<Phi> ` I) \<subseteq> (\<Phi> ` I)"
-  by auto
+text \<open>Now we can directly define the expressiveness function as \<open>direct_expr\<close>.\<close>
 
 function direct_expr :: "('a, 's)hml \<Rightarrow> enat \<times> enat \<times> enat \<times> enat \<times> enat \<times> enat" where
   "direct_expr TT = (0, 1, 0, 0, 0, 0)" |
@@ -66,6 +136,15 @@ function direct_expr :: "('a, 's)hml \<Rightarrow> enat \<times> enat \<times> e
 (Sup ((fst \<circ> snd \<circ> snd \<circ> snd \<circ> snd \<circ> direct_expr \<circ> \<Phi>) ` I \<union> (fst \<circ> snd \<circ> snd \<circ> snd \<circ> snd \<circ> direct_expr \<circ> \<Phi>) ` J \<union> (fst \<circ> direct_expr \<circ> \<Phi>) ` J)), 
 (Sup ((snd \<circ> snd \<circ> snd \<circ> snd \<circ> snd \<circ> direct_expr \<circ> \<Phi>) ` I \<union> ((eSuc \<circ> snd \<circ> snd \<circ> snd \<circ> snd \<circ> snd \<circ> direct_expr \<circ> \<Phi>) ` J))))"
   by ((meson hml.exhaust), simp+)
+
+text \<open>In order to demonstrate termination of the function, it is necessary to establish that each sequence of recursive function calls reaches a base case. 
+This is accomplished by proving that the relation between process-formula pairs, as defined recursively by the function, is contained within a well-founded relation. 
+A relation \( R \subset X \times X \) is considered well-founded if every non-empty subset \( X' \subset X \) contains a minimal element \( m \) such that \( (x, m) \notin R \) for all \( x \in X' \). 
+A key property of well-founded relations is that all descending chains \( (x_0, x_1, x_2, \ldots) \) (where \( (x_i, x_{i+1}) \in R \)) originating from any element \( x_0 \in X \) are finite. 
+Consequently, this ensures that each sequence of recursive invocations terminates after a finite number of steps. 
+
+These proofs were inspired by the Isabelle formalizations presented in [WEP+16].
+\<close>
 
 inductive_set HML_wf_rel :: "(('a, 's)hml) rel" where
 "\<phi> = \<Phi> i \<and> i \<in> (I \<union> J) \<Longrightarrow> (\<phi>, (hml_conj I J \<Phi>)) \<in> HML_wf_rel" |
@@ -96,9 +175,26 @@ proof safe
   qed
 qed
 
+lemma pos_r_subs: "pos_r (\<Phi> ` I) \<subseteq> (\<Phi> ` I)"
+  by auto
+
 termination
   apply rule
   using HML_wf_rel_is_wf HML_wf_rel.simps Un_iff pos_r_subs by fastforce+
+
+text \<open>The other functions are also defined recursively:
+
+Formula nesting depth of conjunctions $\textsf{expr}_2$:
+
+\begin{align*}
+    \text{if } \varphi &= \langle a \rangle \psi \quad \text{ with } a \in \Sigma \\
+    & \text{then } \textsf{expr}_2(\varphi) = \textsf{expr}_2(\psi) \\
+    \text{if } \varphi &= \bigwedge_{i \in I} \{\psi_i \} \\
+    & \text{then } \textsf{expr}_2(\varphi) = 1 + \sup(\textsf{expr}_2(\psi_i)) \\
+    \text{if } \psi &= \neg \varphi \\
+    & \text{then } \textsf{expr}_2(\psi) = \textsf{expr}_2(\varphi)
+\end{align*}
+\<close>
 
 primrec expr_2 :: "('a, 's)hml \<Rightarrow> enat"
   where
@@ -106,6 +202,17 @@ expr_2_tt: \<open>expr_2 TT = 1\<close> |
 expr_2_conj: \<open>expr_2 (hml_conj I J \<Phi>) = 1 + Sup ((expr_2 \<circ> \<Phi>) ` I \<union> (expr_2 \<circ> \<Phi>) ` J)\<close> |
 expr_2_pos: \<open>expr_2 (hml_pos \<alpha> \<phi>) = expr_2 \<phi>\<close>
 
+text \<open>Maximal modal depth of the deepest positive branch $\textsf{expr}_3$:
+
+\begin{align*}
+    \text{if } \varphi &= \langle a \rangle \psi \quad \text{ with } a \in \Sigma \\
+    & \text{then } \textsf{md}(\varphi) = \textsf{md}(\psi) \\
+    \text{if } \varphi &= \bigwedge_{i \in I} \{ \psi_i \} \\
+    & \text{then } \textsf{md}(\varphi) = \sup(\{\textsf{expr}_1(\psi_i) | i \in \text{Pos}\} \cup \{\textsf{expr}_3(\psi_i) | i \in I\}) \\
+    \text{if } \psi &= \neg \varphi \\
+    & \text{then } \textsf{expr}_3(\psi) = \textsf{expr}_3(\varphi)
+\end{align*}
+\<close>
 
 primrec expr_3 :: "('a, 's) hml \<Rightarrow> enat"
   where
@@ -113,11 +220,35 @@ expr_3_tt: \<open>expr_3 TT = 0\<close> |
  expr_3_pos: \<open>expr_3 (hml_pos \<alpha> \<phi>) = expr_3 \<phi>\<close> | 
 expr_3_conj: \<open>expr_3 (hml_conj I J \<Phi>) = (Sup ((expr_1 \<circ> \<Phi>) ` I \<union> (expr_3 \<circ> \<Phi>) ` I \<union> (expr_3 \<circ> \<Phi>) ` J))\<close>
 
+text \<open>Maximal modal depth of other positive clauses in conjunctions $\textsf{expr}_4$:
+
+\begin{align*}
+    \text{if } \varphi &= \langle a \rangle \psi \quad \text{ with } a \in \Sigma \\
+    & \text{then } \textsf{expr}_4(\varphi) = \textsf{expr}_4(\psi) \\
+    \text{if } \varphi &= \bigwedge_{i \in I} \{\ \psi_i \} \\
+    & \text{then } \text{md}(\varphi) = \sup(\{\textsf{expr}_1(\psi_i)|i\in\text{Pos}\backslash \mathcal{R}\}\cup\{\textsf{expr}_4(\psi_i) | i \in I\}) \\
+    \text{if } \psi &= \neg \varphi \\
+    & \text{then } \textsf{expr}_4(\psi) = \textsf{expr}_4(\varphi)
+\end{align*}
+\<close>
+
 primrec expr_4 :: "('a, 's)hml \<Rightarrow> enat" 
   where
 expr_4_tt: "expr_4 TT = 0" |
 expr_4_pos: "expr_4 (hml_pos a \<phi>) = expr_4 \<phi>" |
 expr_4_conj: "expr_4 (hml_conj I J \<Phi>) = Sup ((expr_1 ` (pos_r (\<Phi> ` I)))  \<union> (expr_4 \<circ> \<Phi>) ` I \<union> (expr_4 \<circ> \<Phi>) ` J)"
+
+text \<open>Maximal modal depth of negative clauses in conjunctions $\textsf{expr}_5$:
+
+\begin{align*}
+    \text{if } \varphi &= \langle a \rangle \psi \quad \text{ with } a \in \Sigma \\
+    & \text{then } \textsf{expr}_5(\varphi) = \textsf{expr}_5(\psi) \\
+    \text{if } \varphi &= \bigwedge_{i \in I} \{ \psi_i \} \\
+    & \text{then } \textsf{expr}_5(\varphi) = \sup(\{\textsf{expr}_1(\psi_i)| i \in \text{Neg}\}\cup \{\textsf{expr}_5(\psi_i)|i \in I\}) \\
+    \text{if } \psi &= \neg \varphi \\
+    & \text{then } \textsf{expr}_5(\psi) = \textsf{expr}_5(\varphi)
+\end{align*}
+\<close>
 
 primrec expr_5 :: "('a, 's)hml \<Rightarrow> enat"
   where
@@ -126,6 +257,18 @@ expr_5_pos:\<open>expr_5 (hml_pos \<alpha> \<phi>) = expr_5 \<phi>\<close>|
 expr_5_conj: \<open>expr_5 (hml_conj I J \<Phi>) = 
 (Sup ((expr_5 \<circ> \<Phi>) ` I \<union> (expr_5 \<circ> \<Phi>) ` J \<union> (expr_1 \<circ> \<Phi>) ` J))\<close>
 
+text \<open>Formula nesting depth of negations $\textsf{expr}_6$:
+
+\begin{align*}
+    \text{if } \varphi &= \langle a \rangle \psi \quad \text{ with } a \in \Sigma \\
+    & \text{then } \textsf{expr}_6(\varphi) = \textsf{expr}_6(\psi) \\
+    \text{if } \varphi &= \bigwedge_{i \in I} \{ \psi_i \} \\
+    & \text{then } \textsf{expr}_6(\varphi) = \sup(\{\textsf{expr}_6(\psi_i)| i \in I\}) \\
+    \text{if } \psi &= \neg \varphi \\
+    & \text{then } \textsf{expr}_6(\psi) = 1 + \textsf{expr}_6(\varphi)
+\end{align*}
+\<close>
+
 primrec expr_6 :: "('a, 's)hml \<Rightarrow> enat"
   where
 expr_6_tt: \<open>expr_6 TT = 0\<close> |
@@ -133,21 +276,16 @@ expr_6_pos: \<open>expr_6 (hml_pos \<alpha> \<phi>) = expr_6 \<phi>\<close>|
 expr_6_conj: \<open>expr_6 (hml_conj I J \<Phi>) = 
 (Sup ((expr_6 \<circ> \<Phi>) ` I \<union> ((eSuc \<circ> expr_6 \<circ> \<Phi>) ` J)))\<close>
 
+text \<open>That leaves us with a definition \textsf{expr} of the expressiveness function that is easier to use.\<close>
 
 fun expr :: "('a, 's)hml \<Rightarrow> enat \<times> enat \<times> enat \<times>  enat \<times> enat \<times> enat" 
   where
 \<open>expr \<phi> = (expr_1 \<phi>, expr_2 \<phi>, expr_3 \<phi>, expr_4 \<phi>, expr_5 \<phi>, expr_6 \<phi>)\<close>
 
-lemma apply_comp:
-  assumes "\<forall>x \<in> \<Phi> ` I. F x = G1 (G2 (G3 (G4 (G5 ((H x))))))"
-  shows "Sup ((F \<circ> \<Phi>) ` I) = Sup((G1 \<circ> G2 \<circ> G3 \<circ> G4 \<circ> G5 \<circ> H \<circ> \<Phi>) ` I)"
-  using assms by auto
+text \<open>We show that \<open>direct_expr\<close> and \<open>expr\<close> are the same:\<close>
 
-lemma fa_set_eq: 
-  assumes "\<forall>x \<in> \<Phi> ` I. F x = G (H x)"
-  shows "((F \<circ> \<Phi>) ` I) = (G \<circ> H \<circ> \<Phi>) ` I" 
-  using assms by force
 
+(*<*)
 lemma expr_6_direct_expr_eq:
   assumes "\<And>x. x \<in> \<Phi> ` I \<Longrightarrow> expr_6 x = snd (snd (snd (snd (snd (direct_expr x)))))"
   shows "(expr_6 \<circ> \<Phi>) ` I = (snd \<circ> snd \<circ> snd \<circ> snd \<circ> snd \<circ> direct_expr \<circ> \<Phi>) ` I"
@@ -184,8 +322,7 @@ proof-
     by blast
   finally show ?thesis.
 qed
-
-thm comp_apply
+(*>*)
 
 lemma 
   shows "expr \<phi> = direct_expr \<phi>"
